Build up more infrastructure towards proof of correctness

dafny/def.dfy
@@ -12,6 +12,7 @@ import opened Wrappers
 ////////////////////////////////////////
 datatype Term = Var(s:string) | Const(c:string) 
 type ConstTerm = t:Term | t.Const? witness Const("")
+type VarTerm = t:Term | t.Var? witness Var("")
 type Substitution = map<Term,ConstTerm>
 datatype Clause = Clause(name:string, terms:seq<Term>)
 {
@@ -162,10 +163,45 @@ predicate valid_program(p:Program) {
   forall i :: 0 <= i < |p| ==> valid_rule(p[i])
 }
 
+function apply_sub(c:Clause, sub:Substitution) : Clause
+{
+  var new_terms := 
+      seq(|c.terms|, 
+          i requires 0 <= i < |c.terms| => 
+            var t := c.terms[i];
+            match t
+              case Const(_) => t
+              case Var(_) => if t in sub then sub[t] else t);
+    Clause(c.name, new_terms)
+}
+
+// Needed below to satisfy Dafny's type checker
+function term_to_var_term(t:Term) : VarTerm
+  requires t.Var?
+{
+  t
+}
+
+function terms_vars(terms:seq<Term>) : set<VarTerm>
+{
+  set i | 0 <= i < |terms| && terms[i].Var? :: term_to_var_term(terms[i])
+}
+
+function clause_vars(c:Clause) : set<VarTerm>
+{
+  terms_vars(c.terms)
+}
+/*
+function clauses_vars(clauses:seq<Clause>) : set<VarTerm>
+{
+  set i | 0 <= i < |clauses| && clauses[i].Var? :: clauses
+}
+*/
 method substitute(c:Clause, sub:Substitution) returns (c':Clause)
   ensures c.substitution_complete(sub) ==> c'.is_ground()
   ensures forall sub' :: c'.substitution_complete(sub') ==>
             c.substitution_complete(sub + sub')
+  ensures c' == apply_sub(c, sub)
 {
   var new_terms := 
     seq(|c.terms|, 
@@ -195,6 +231,7 @@ method unify_terms(terms:seq<Term>, consts:seq<ConstTerm>) returns (s:Option<Sub
       match terms[j]
         case Var(_) => terms[j] in s.value && s.value[terms[j]] == consts[j]
         case Const(_) => terms[j] == consts[j])
+    && s.value.Keys == terms_vars(terms)
 {
   if |terms| != |consts| {
     s := None;
@@ -203,7 +240,11 @@ method unify_terms(terms:seq<Term>, consts:seq<ConstTerm>) returns (s:Option<Sub
   } else {
     var sub:Substitution := map[];
     for i := 0 to |terms| 
-      invariant forall j :: 0 <= j < i ==> (terms[j].Var? ==> terms[j] in sub && sub[terms[j]] == consts[j])
+      invariant sub.Keys == terms_vars(terms[..i])
+      invariant forall j :: 0 <= j < i ==> 
+        match terms[j]
+        case Var(_) => terms[j] in sub && sub[terms[j]] == consts[j]
+        case Const(_) => terms[j] == consts[j]
     {
       var term := terms[i];
       var cons := consts[i];
@@ -226,7 +267,9 @@ method unify_terms(terms:seq<Term>, consts:seq<ConstTerm>) returns (s:Option<Sub
 }
 
 method unify(c:Clause, fact:Fact) returns (s:Option<Substitution>)
-  ensures s.Some? ==> c.substitution_complete(s.value) && c.make_fact(s.value) == fact
+  ensures s.Some? ==> c.substitution_complete(s.value) 
+                   && c.make_fact(s.value) == fact
+                   && s.value.Keys == clause_vars(c)
 {
   if c.name != fact.name {
     return None;
@@ -246,6 +289,41 @@ predicate facts_complete_all(c:Clause, subs:seq<Substitution>, kb:KnowledgeBase)
   requires subs_complete_all(c, subs)
 {
   forall m :: 0 <= m < |subs| ==> c.make_fact(subs[m]) in kb
+}
+
+lemma lemma_make_fact_consistent(c:Clause, f:Fact, s:Substitution, s0:Substitution, s1:Substitution)
+  requires s == s0 + s1
+  requires c.substitution_complete(s1)
+  requires c.make_fact(s1) == f
+  ensures  c.make_fact(s) == f
+{
+
+}
+
+lemma make_fact_transitive(c:Clause, g:Clause, fact:Fact, s0:Substitution, s1:Substitution)
+  requires g == apply_sub(c, s0)
+  requires g.substitution_complete(s1)
+  requires s1.Keys == clause_vars(g)
+  requires fact == g.make_fact(s0 + s1)
+  ensures  c.substitution_complete(s0 + s1)
+  ensures  fact == c.make_fact(s0 + s1)
+{
+  var s := s0 + s1;
+  assert c.substitution_complete(s) by {
+    forall t | t in c.terms && t.Var?
+      ensures t in s
+    {
+      if t in g.terms {
+        assert t in s1;
+      } else {
+        if t !in s0 {
+          var i :| 0 <= i < |c.terms| && c.terms[i] == t;
+          assert g.terms[i] == if t in s0 then s0[t] else t;
+        }
+        
+      }
+    }
+  }  
 }
 
 method eval_clause(kb:KnowledgeBase, c:Clause, subs:seq<Substitution>) returns (subs':seq<Substitution>)
@@ -274,19 +352,50 @@ method eval_clause(kb:KnowledgeBase, c:Clause, subs:seq<Substitution>) returns (
         case None =>
         case Some(sub) =>
           assert grounded.substitution_complete(sub);
-          assert grounded.make_fact(sub) == kb[j];
+ 
+          //assume sub.Keys * subs[i].Keys == {};
+          //assert grounded.make_fact(sub + subs[i]) == kb[j];
           //print "\t\tUnified ", c, " with ", kb[j], " and got ", sub, "\n";
           ghost var old_subs' := subs';
-          subs' := subs' + [sub + subs[i]];
+          subs' := subs' + [subs[i] + sub];
+          //assert Last(subs') == subs[i] + sub;
+          forall k | 0 <= k < |subs'|
+            ensures c.substitution_complete(subs'[k]) && c.make_fact(subs'[k]) in kb
+          {            
+            if k < |subs'| - 1 {
+              assert subs'[k] == old_subs'[k];
+              assert c.make_fact(subs'[k]) in kb;
+            } else {
+              assert subs'[k] == subs[i] + sub;
+              assert grounded.make_fact(sub) == kb[j];
+              lemma_make_fact_consistent(grounded, kb[j], subs[i] + sub, subs[i], sub);
+              assert grounded.make_fact(subs[i] + sub) == kb[j];
+              make_fact_transitive(c, grounded, kb[j], subs[i], sub);
+            }          
+          }
+        forall c':Clause | subs_complete_all(c', subs) && facts_complete_all(c', subs, kb) 
+          ensures subs_complete_all(c', subs') && facts_complete_all(c', subs', kb)
+        {
+          forall m | 0 <= m < |subs'|
+            ensures c'.make_fact(subs'[m]) in kb
+          {
+            if m < |old_subs'| {
+            } else {              
+              //assume sub.Keys * subs[i].Keys == {};
+              assert subs'[m] == subs[i] + sub;
+              assert c'.make_fact(subs'[m]) == c'.make_fact(subs[i]);
+            }
+          }
+        }
       }
     }
   }
 }
 
-method eval_clauses(kb:KnowledgeBase, clauses:seq<Clause>) returns (subs:seq<Substitution>)
-  ensures forall k, j :: 0 <= k < |subs| && 0 <= j < |clauses| ==> 
-                 clauses[j].substitution_complete(subs[k])
-              && clauses[j].make_fact(subs[k]) in kb;
+method eval_clauses(kb:KnowledgeBase, clauses:seq<Clause>) returns (subs:seq<Substitution>) 
+  ensures forall j :: 0 <= j < |clauses| ==> 
+              && subs_complete_all(clauses[j], subs)
+              && facts_complete_all(clauses[j], subs, kb)
 {
   subs := [map[]];
   for i := 0 to |clauses| 
@@ -299,9 +408,9 @@ method eval_clauses(kb:KnowledgeBase, clauses:seq<Clause>) returns (subs:seq<Sub
   }
 }
 
-predicate valid_partial_proof(prog:Program, facts:set<Fact>, query:Rule, proof:Proof)
+predicate valid_partial_proof(prog:Program, facts:set<Fact>, proof:Proof)
 {
-  && |proof| > 0
+  |proof| > 0 ==>
   // We start with the base set of facts
   && First(proof).facts == facts
   // Each proof step is valid and uses a rule from the program
@@ -310,22 +419,46 @@ predicate valid_partial_proof(prog:Program, facts:set<Fact>, query:Rule, proof:P
   && (forall i :: 0 <= i < |proof| - 1 ==> proof[i+1].facts == proof[i].facts + { proof[i].new_fact() } )
 }
 
-method eval_rule(kb:KnowledgeBase, r:Rule) returns (kb':KnowledgeBase)
-  requires valid_rule(r)
+lemma lemma_valid_proof_step(step:ProofStep)
+  requires valid_rule(step.rule)
+  requires forall j :: 0 <= j < |step.rule.body| ==>                 
+                 step.rule.body[j].substitution_complete(step.sub)
+              && step.rule.body[j].make_fact(step.sub) in step.facts
+  ensures step.valid()
 {
+  assume false;
+}
+
+method eval_rule(kb:KnowledgeBase, r:Rule) returns (kb':KnowledgeBase, ghost proof:Proof)
+  requires valid_rule(r)
+  ensures |proof| == |kb'|
+  ensures forall j :: 0 <= j < |proof| ==> 
+              proof[j].valid() && proof[j].rule == r && proof[j].facts == ToSet(kb)
+  ensures forall j :: 0 <= j < |kb'| ==>  kb'[j] == proof[j].rule.head.make_fact(proof[j].sub)
+{
+  proof := [];
   //print "Evaluating rule: ", r, "\n";
   if |r.body| == 0 {
-    return [r.head];
+    return [r.head], [ProofStep(map[], r, ToSet(kb))];
   }
 
   kb' := [];
+
   var subs := eval_clauses(kb, r.body);
   //print "\teval_clauses returned: ", subs, "\n";
-  for i := 0 to |subs| {
+  for i := 0 to |subs| 
+    invariant |proof| == |kb'| == i
+    invariant forall j :: 0 <= j < |proof| ==> 
+              proof[j].valid() && proof[j].rule == r && proof[j].facts == ToSet(kb)
+    invariant forall j :: 0 <= j < i ==>  kb'[j] == proof[j].rule.head.make_fact(proof[j].sub)       
+  {
     var new_fact := substitute(r.head, subs[i]);
     //print "\tFound a new fact: ", new_fact, "\n";
-    // TODO:
-    //assume new_fact.is_ground();
+    ghost var step := ProofStep(subs[i], r, ToSet(kb));  
+    assert forall f :: f in kb ==> f in ToSet(kb) by { reveal ToSet(); }    
+    lemma_valid_proof_step(step);
+    assert step.valid();
+    proof := proof + [step];
     kb' := kb' + [new_fact];
   }
 }
@@ -345,6 +478,7 @@ method LemmaHasNoDuplicatesExtend<T>(s:seq<T>, elt:T)
 method SetToSeq<T>(s:set<T>) returns (q:seq<T>)
   ensures HasNoDuplicates(q)
   ensures |q| == |s|
+  ensures ToSet(q) == s
 {
   q := [];
   var subset := s;
@@ -369,6 +503,7 @@ method merge(kb0:KnowledgeBase, kb1:KnowledgeBase) returns (kb':KnowledgeBase)
   requires HasNoDuplicates(kb0)
   ensures HasNoDuplicates(kb')
   ensures |kb'| >= |kb0|
+  ensures ToSet(kb') == ToSet(kb0) + ToSet(kb1)
 {
   var s0 := ToSet(kb0);
   var s1 := ToSet(kb1);
@@ -380,36 +515,65 @@ method merge(kb0:KnowledgeBase, kb1:KnowledgeBase) returns (kb':KnowledgeBase)
   kb' := SetToSeq(union);
 }
 
-method immediate_consequence(prog:Program, kb:KnowledgeBase) returns (kb':KnowledgeBase)
+ghost method merge_proofs(prog:Program, initial_facts:set<Fact>, proof:Proof, proof_steps:Proof, old_kb:KnowledgeBase, new_kb:KnowledgeBase) 
+  returns (proof':Proof)
+  requires valid_partial_proof(prog, initial_facts, proof)
+  requires |proof| > 0 ==> Last(proof).facts == ToSet(old_kb);
+  requires |proof_steps| == |new_kb|
+  requires forall j :: 0 <= j < |proof_steps| ==> 
+              proof_steps[j].valid() && proof_steps[j].rule in prog && proof_steps[j].facts == ToSet(old_kb)
+  requires forall j :: 0 <= j < |new_kb| ==>  new_kb[j] == proof_steps[j].rule.head.make_fact(proof_steps[j].sub)
+  ensures |proof'| > |proof|
+  ensures Last(proof').facts == ToSet(old_kb) + ToSet(new_kb)
+  ensures valid_partial_proof(prog, initial_facts, proof')
+{
+  assume false;
+}
+
+method immediate_consequence(prog:Program, kb:KnowledgeBase, ghost initial_facts:set<Fact>, ghost proof:Proof)
+  returns (kb':KnowledgeBase, ghost proof':Proof)
   requires valid_program(prog)
   requires HasNoDuplicates(kb)
+  requires valid_partial_proof(prog, initial_facts, proof)
+  requires |proof| > 0 ==> Last(proof).facts == ToSet(kb)
   ensures HasNoDuplicates(kb')
   ensures |kb'| >= |kb|
+  ensures valid_partial_proof(prog, initial_facts, proof')
+  ensures |proof'| > 0 ==> Last(proof').facts == ToSet(kb')
 {
   kb' := kb;
+  proof' := proof;
   for i := 0 to |prog| 
     invariant HasNoDuplicates(kb')
     invariant |kb'| >= |kb|
+    invariant valid_partial_proof(prog, initial_facts, proof')
+    invariant |proof'| > 0 ==> Last(proof').facts == ToSet(kb')
   {
-    var new_kb := eval_rule(kb', prog[i]);
+    var new_kb, proof_steps := eval_rule(kb', prog[i]);
+    proof' := merge_proofs(prog, initial_facts, proof', proof_steps, kb', new_kb);    
     kb' := merge(kb', new_kb);    
   }
 }
 
-method solve(prog:Program) returns (kb:KnowledgeBase)
+method solve(prog:Program) returns (kb:KnowledgeBase, ghost proof:Proof)
   requires valid_program(prog)
+  ensures valid_partial_proof(prog, ToSet([]), proof)
+  ensures |proof| > 0 ==> Last(proof).facts == ToSet(kb)
 {
   kb := [];
-  LemmaCardinalityOfEmptySetIs0(kb);
+  proof := [];
+  LemmaCardinalityOfEmptySetIs0(kb);  
   LemmaNoDuplicatesCardinalityOfSet(kb);
   var count := 4294967295;  // Cheap hack to avoid proving termination
   while count > 0 
     invariant HasNoDuplicates(kb)
+    invariant valid_partial_proof(prog, ToSet([]), proof)
+    invariant |proof| > 0 ==> Last(proof).facts == ToSet(kb)
   {
     var old_kb := kb;
-    kb := immediate_consequence(prog, old_kb);
+    kb, proof := immediate_consequence(prog, old_kb, ToSet([]), proof);
     if |kb| == |old_kb| {
-      return kb;
+      return kb, proof;
     }
     count := count - 1;
   }
@@ -482,11 +646,33 @@ method check_program(prog:Program) returns (b:bool)
   }
 }
 
+// Checks if any fact can satisfy the query
 method query(prog:Program, query:Rule)
   requires valid_program(prog)
   requires valid_rule(query)
 {  
-  var kb := solve(prog + [query]);
+  var kb, partial_proof := solve(prog);
+  assert valid_partial_proof(prog, ToSet([]), partial_proof);
+  var new_kb, proof_steps := eval_rule(kb, query);
+  assume false;
+  var proof := merge_proofs(prog, ToSet([]), partial_proof, proof_steps, kb, new_kb);    
+  //kb' := merge(kb', new_kb);
+  if |new_kb| > 0 {
+    assert valid_proof(prog, ToSet([]), query, proof);
+  }
+  
+  print "Done\n";
+}
+
+// Finds all facts derivable from the query
+method query_all(prog:Program, query:Rule)
+  requires valid_program(prog)
+  requires valid_rule(query)
+{  
+  var kb, proof := solve(prog + [query]);
+  //if ? {
+  //  assert valid_proof(prog, ToSet([]), query, proof);
+  //}
   print "Results:\n";
   for i := 0 to |kb| {
     //print kb[i], "\n";
@@ -508,7 +694,7 @@ method run(raw_prog:Program)
   var valid_prog := check_program(prog);
   var valid_query := check_rule(q);
   if valid_prog && valid_query {
-    query(prog, q);  
+    query_all(prog, q);  
   } else {
     print "Sorry, that's an invalid program and/or query\n";
   }
